theories/FOL/Completeness2/KripkeCompleteness.v
@@ -1,0 +1,352 @@
+(** ** Completeness **)
+
+From Undecidability.FOL Require Import Syntax.Facts Deduction.FragmentNDFacts Syntax.Theories Semantics.Kripke.FragmentCore Semantics.Kripke.FragmentSoundness 
+                                       Semantics.Kripke.FragmentToTarski Deduction.FragmentSequent Deduction.FragmentSequentFacts.
+From Undecidability.Synthetic Require Import Definitions DecidabilityFacts EnumerabilityFacts ListEnumerabilityFacts ReducibilityFacts.
+From Undecidability Require Import Shared.ListAutomation Shared.Dec.
+From Undecidability Require Import Shared.Libs.PSL.Vectors.Vectors Shared.Libs.PSL.Vectors.VectorForall.
+Import ListAutomationNotations.
+From Undecidability.FOL.Completeness2 Require Export TarskiCompleteness.
+(* From Undecidability.FOLC Require Export Gentzen. *)
+
+(* *** Exploding and Minimal Models *)
+
+Section KripkeCompleteness.
+  Context {Σf : funcs_signature} {Σp : preds_signature}. (*
+  Variable eF : nat -> option Σf.
+  Context {HeF : enumerator__T eF Σf}.
+  Variable eP : nat -> option Σp.
+  Context {HeP : enumerator__T eP Σp}. *)
+
+(*  Hint Constructors sprv. *)
+  Instance model_bot : interp term :=
+    {| i_func := func; i_atom := fun P v => False|}.
+  Lemma universal_interp_eval rho t :
+    eval rho t = t`[rho].
+  Proof.
+    now induction t; cbn.
+  Qed.
+
+  Section Contexts.
+
+    Program Instance K_ctx {ff:falsity_flag} : kmodel term :=
+      {|
+        nodes := list form ;
+        reachable := @incl form ;
+        k_interp := model_bot ;
+        k_P := fun A P v => sprv A None (atom P v) ;
+      |}.
+    Next Obligation.
+      abstract (intuition; now apply (incl_tran H)).
+    Qed.
+    Next Obligation.
+      abstract (eauto using seq_Weak).
+    Qed.
+
+    Definition F_P {ff} : list (@form _ _ _ ff) -> Prop := match ff with falsity_on => fun n => sprv n None ⊥ | _ => fun _ => False end.
+    Lemma mon_F {ff:falsity_flag} (u v : @nodes _ _ _ K_ctx) : reachable u v -> F_P u -> F_P v.
+    Proof.
+      cbn. unfold F_P. destruct ff; try easy. intros H H1. eapply seq_Weak; [ exact H1| exact H].
+    Qed.
+
+    Notation "rho '⊩⊥(' u , M ')' phi" :=  (@ksat_bot _ _ _ M _ F_P mon_F u rho phi) (at level 20).
+
+    Lemma K_ctx_correct {ff:falsity_flag} (A : list form) rho phi :
+      (rho ⊩⊥(A, K_ctx ) phi-> A ⊢S phi[rho]) /\
+      ((forall B psi, A <<= B -> B ;; phi[rho] ⊢s psi -> B ⊢S psi) -> rho ⊩⊥(A, K_ctx) phi).
+    Proof.
+      revert A rho; enough ((forall A rho, rho ⊩⊥( A, K_ctx) phi -> A ⊢S phi[rho]) /\
+                          (forall A rho, (forall B psi, A <<= B -> B;; phi[rho] ⊢s psi -> B ⊢S psi)
+                                  -> rho ⊩⊥( A, K_ctx) phi)) by intuition.
+      induction phi as [|t1 t2|ff [] phi IHphi psi IHpsi|ff [] phi IHphi]; cbn; split; intros A rho.
+      - tauto.
+      - eauto.
+      - erewrite Vector.map_ext. 1: eauto. apply universal_interp_eval.
+      - intros H. erewrite Vector.map_ext. 1: now apply H. apply universal_interp_eval.
+      - intros Hsat. apply IR, IHpsi. apply Hsat, IHphi. 1: intuition. eauto.
+      - intros H B HB Hphi % IHphi. apply IHpsi. intros C xi HC Hxi. apply H.
+        1: now transitivity B. eauto using seq_Weak.
+      - intros Hsat. apply AllR.
+        pose (phi' := subst_form ($0 .: (rho >> subst_term (S >> var))) phi).
+        destruct (find_bounded_L (phi' :: A)).
+        eapply seq_nameless_equiv_all' with (n := x) (phi := phi').
+        + intros xi Hxi. apply b. now right.
+        + eapply bounded_up. 1: apply b; now left. lia.
+        + unfold phi'. rewrite subst_comp. erewrite subst_ext.
+          * eapply IHphi. apply Hsat.
+          * intros [|n]; cbn. 1:reflexivity.
+            unfold funcomp. rewrite subst_term_comp. apply subst_term_id.
+            intros [|m]; easy.
+      - intros H t. apply IHphi. intros B psi HB Hpsi. apply H. assumption.
+        apply AllL with (t := t). now rewrite help5.
+    Qed.
+
+    Corollary K_ctx_sprv {ff:falsity_flag} A rho phi :
+      rho ⊩⊥(A, K_ctx) phi -> A ⊢S phi[rho].
+    Proof.
+      now destruct (K_ctx_correct A rho phi).
+    Qed.
+
+    Lemma K_ctx_subst {ff:falsity_flag} A phi rho :
+      rho ⊩⊥( A, K_ctx) phi <-> var ⊩⊥( A, K_ctx) phi[rho].
+    Proof.
+      unfold ksat_bot, falsity_to_pred.
+      rewrite <- atom_subst_comp_strong. 2:easy.
+      assert (forall {ff:falsity_flag} rho, (atom (Σ_preds := Σ_preds_bot) (inl tt) (Vector.nil _)) = (atom (Σ_preds := Σ_preds_bot) (inl tt) (Vector.nil _))[rho]) as Heq by easy.
+      erewrite Heq.
+      rewrite <- subst_falsity_comm. cbn.
+      rewrite (ksat_comp A var rho).
+      apply ksat_ext. intros x. unfold funcomp. induction (rho x); cbn; try easy.
+      erewrite <- map_ext_forall. 2: apply Forall_in, IH. 
+      now rewrite Vector.map_id.
+    Qed.
+
+    Lemma K_ctx_constraint {ff:falsity_flag} A rho psi:
+      rho ⊩⊥(A, K_ctx) (⊥ → psi).
+    Proof.
+      destruct ff eqn : Hff; try now intros.
+      intros v B HB. cbn in HB. apply K_ctx_correct.
+      intros B' psi' HB' Hprv. subst. eauto using seq_Weak.
+    Qed.
+
+
+
+  Ltac clean_ksoundness :=
+    match goal with
+    | [ H : ?x = ?x -> _ |- _ ] => specialize (H eq_refl)
+    | [ H : (?A -> ?B), H2 : (?A -> ?B) -> _ |- _] => specialize (H2 H)
+    end.
+
+  Lemma ksoundness_f2p_model {ff1 ff2 : falsity_flag} A phi:
+    A ⊢I phi -> 
+    forall u rho, 
+    (forall psi', psi' el A -> rho ⊩⊥(u,K_ctx) psi') -> 
+    rho ⊩⊥(u,K_ctx) phi.
+  Proof.
+    intros Hprv. remember intu as s. induction Hprv; subst; cbn; intros u rho HA.
+    all: repeat (clean_ksoundness + discriminate). all: (eauto || cbn -[F_P]; eauto).
+    - intros v Hr Hpi. eapply IHHprv. intros ? []; subst; eauto using ksat_mon. eapply ksat_mon. 2: now apply HA. easy.
+    - eapply IHHprv1. 3: eapply IHHprv2. all: eauto. apply K_ctx.
+    - intros d. apply IHHprv. intros psi [psi' [<- Hp]] % in_map_iff. cbn.
+      unfold ksat_bot. rewrite falsity_to_pred_subst.
+      rewrite ksat_comp. apply HA, Hp.
+    - unfold ksat_bot. rewrite falsity_to_pred_subst.
+      rewrite ksat_comp. eapply ksat_ext. 2: eapply (IHHprv u rho HA (eval rho t)). 
+      unfold funcomp. now intros [].
+    - apply (@K_ctx_constraint _ u rho phi). 1:reflexivity.
+      cbn. apply (IHHprv u rho). apply HA.
+  Qed.
+
+    Fact K_ctx_sprv' {ff:falsity_flag}  A rho phi :
+      A ⊢S phi[rho] -> rho ⊩⊥(A, K_ctx) phi.
+    Proof.
+      intros H % seq_ND. apply K_ctx_subst.
+      eapply ksoundness_f2p_model.
+      - apply H.
+      - cbn in H. intros psi HP. apply K_ctx_correct.
+        intros B theta H1 H2. eapply Contr; eauto.
+        rewrite subst_id. 1: now apply H1. easy.
+    Qed.
+
+    Corollary K_ctx_ksat {ff:falsity_flag} A rho phi :
+      (forall B psi, A <<= B -> B ;; phi[rho] ⊢s psi -> B ⊢S psi) -> rho ⊩⊥(A, K_ctx) phi.
+    Proof.
+      now destruct (K_ctx_correct A rho phi).
+    Qed.
+  End Contexts.
+(*
+  Section ExplodingCompleteness.
+
+    Lemma K_ctx_exploding :
+      kexploding (@K_ctx expl).
+    Proof.
+      apply (@K_ctx_constraint expl).
+    Qed.
+
+    Lemma K_exp_completeness A phi :
+      A ⊫KE phi -> A ⊢SE phi.
+    Proof.
+      intros Hsat. erewrite <-idSubst_form. apply K_ctx_sprv with (rho := ids). 2: reflexivity.
+      apply Hsat. 1: apply K_ctx_exploding. intros psi Hpsi. apply K_ctx_ksat. intros B xi HB Hxi.
+      asimpl in Hxi. eauto.
+    Qed.
+
+    Lemma K_exp_seq_ksoundness A phi :
+      A ⊢SE phi -> A ⊫KE phi.
+    Proof.
+      intros H % seq_ND. apply @ksoundness with (b := expl). 2: apply H. firstorder.
+    Qed.
+
+    Fact SE_cut A phi psi :
+      A ⊢SE phi -> A;;phi ⊢sE psi -> A ⊢SE psi.
+    Proof.
+      intros H1 % seq_ND H2 % seq_ND; cbn in *.
+      apply H2 in H1. apply K_exp_completeness.
+      apply @ksoundness with (b := expl); firstorder.
+    Qed.
+    
+  End ExplodingCompleteness. *)
+
+  Section BottomlessCompleteness.
+    #[local] Existing Instance falsity_off | 0.
+    Lemma K_bottomless_completeness A phi :
+      True -> A ⊢ phi.
+    Proof.
+      intros Hsat. erewrite <-idSubst_form. apply K_ctx_sprv with (rho := ids). 2: reflexivity.
+      apply Hsat. 1: apply I. intros psi Hpsi. apply K_ctx_ksat. intros B xi HB Hxi.
+      asimpl in Hxi. eauto.
+    Qed.
+  End BottomlessCompleteness.
+
+(* *** Standard Models *)
+
+  Section StandardCompleteness.
+    Context {HdF : eq_dec Funcs} {HdP : eq_dec Preds}.
+    Context {HeF : enumT Funcs} {HeP : enumT Preds}.
+
+    Definition cons A := ~ A ⊢SE ⊥.
+    Definition cons_ctx := { A | cons A }.
+    Definition ctx_incl (A B : cons_ctx) := incl (proj1_sig A) (proj1_sig B).
+
+    Hint Unfold cons cons_ctx ctx_incl.
+
+    Notation "A <<=C B" := (ctx_incl A B) (at level 20).
+    Notation "A ⊢SC phi" := (proj1_sig A ⊢SE phi) (at level 20).
+    Notation "A ;; psi ⊢sC phi" := (proj1_sig A ;; psi ⊢sE phi) (at level 20).
+
+    Ltac dest_con_ctx :=
+      match goal with
+      | [ |- forall u : cons_ctx, _] => let Hu := fresh "H" u in intros [u Hu]
+      | [ A : cons_ctx |- _] => let HA := fresh "H" A in destruct A as [A HA]
+      end.
+
+    Ltac cctx := repeat (progress dest_con_ctx); comp.
+
+    Hint Extern 1 => cctx.
+
+    Program Instance K_std : kmodel term :=
+      {|
+        reachable := ctx_incl ;
+        k_interp := universal_interp ;
+        k_P := fun A P v => ~ ~ A ⊢SC (Pred P v) ;
+        k_Bot := fun _ => False
+      |}.
+    Next Obligation.
+      abstract (cctx; firstorder).
+    Qed.
+    Next Obligation.
+      intros H2. apply H0. intros H3. apply H2.
+      abstract (eauto using seq_Weak).
+    Qed.
+
+    Lemma K_std_standard :
+      kstandard K_std.
+    Proof.
+      intros []. cbn. trivial.
+    Qed.
+
+    Lemma K_std_correct (A : cons_ctx) rho phi :
+      (rho ⊩(A, K_std) phi -> ~ ~ A ⊢SC phi[rho]) /\
+      ((forall B psi, A <<=C B -> B ;; phi[rho] ⊢sC psi -> ~ ~ B ⊢SC psi) -> rho ⊩(A, K_std) phi).
+    Proof.
+      revert A rho; enough ((forall A rho, rho ⊩( A, K_std) phi -> ~ ~ A ⊢SC phi[rho])
+                          /\ (forall A rho, (forall B psi, A <<=C B -> B;; phi[rho] ⊢sC psi -> ~ ~ B ⊢SC psi)
+                                    -> rho ⊩( A, K_std) phi)) by firstorder.
+      induction phi as [| t1 t2 | phi [IHphi1 IHphi2] psi [IHpsi1 IHpsi2] | phi [IHphi1 IHphi2]].
+      all: cbn; asimpl; split; intros A rho.
+      - tauto.
+      - intros H. exfalso. apply (H A ⊥); auto.
+      - now rewrite (vec_ext (fun x => universal_interp_eval rho x)).
+      - rewrite (vec_ext (fun x => universal_interp_eval rho x)). intros H H'.
+        eapply H. 3: { intros H1. apply H', H1. } all: auto.
+      - intros Hsat H.
+        assert (HA : ~ ~ ((phi[rho] :: proj1_sig A) ⊢SE ⊥ \/ ~ (phi[rho] :: proj1_sig A) ⊢SE ⊥)) by tauto.
+        apply HA. clear HA. intros [HA|HA].
+        + apply H. apply IR. apply Absurd. assumption.
+        + pose (A' := exist cons (phi[rho] :: proj1_sig A) HA). apply (IHpsi1 A' rho).
+          * apply Hsat; auto 3. apply IHphi2. intros B theta HB HT.
+            intros H'. apply H'. eauto.
+          * intros H'. apply H. apply IR, H'.
+      - intros H B HB Hphi % IHphi1. apply IHpsi2. intros C xi HC Hxi.
+        intros HX. apply Hphi. intros Hphi'. apply (H C xi); trivial.
+        + cctx. now transitivity B.
+        + apply IL; trivial. eapply seq_Weak; eauto.
+      - pose (phi' := subst_form (var_term 0 .: (rho >> subst_term (S >> var_term))) phi).
+        intros Hsat. intros H. cctx. destruct (find_unused_L (phi' :: A)).
+        apply (IHphi1 (exist cons A HA) (var_term x.:rho)).
+        rewrite ksat_ext. 2: reflexivity. now apply Hsat.
+        intros H'. apply H, AllR.
+        eapply seq_nameless_equiv with (n := x) (phi0 := phi').
+        + intros xi Hxi. apply u. constructor. intuition.
+        + apply u. omega. intuition.
+        + unfold phi'. asimpl. apply H'.
+      - intros H t. apply IHphi2. intros B psi HB Hpsi. apply H. assumption.
+        apply AllL with (t0 := t). now asimpl in *.
+    Qed.
+
+    Corollary K_std_sprv A rho phi :
+      rho ⊩(A, K_std) phi -> ~ ~ A ⊢SC phi[rho].
+    Proof.
+      now destruct (K_std_correct A rho phi).
+    Qed.
+
+    Corollary K_std_sprv' A rho phi :
+       ~ ~ A ⊢SC phi[rho] -> rho ⊩(A, K_std) phi.
+    Proof.
+      intros H. apply (K_std_correct A rho phi).
+      intros B psi H1 H2 H3. apply H. intros H'.
+      apply H3. eapply SE_cut; try eassumption.
+      now apply (seq_Weak H').
+    Qed.
+
+    Corollary K_std_ksat A rho phi :
+      (forall B psi, A <<=C B -> B ;; phi[rho] ⊢sC psi -> ~ ~ B ⊢SC psi) -> rho ⊩(A, K_std) phi.
+    Proof.
+      now destruct (K_std_correct A rho phi).
+    Qed.
+
+    Lemma K_std_completeness A phi :
+      A ⊫KS phi -> ~ ~ A ⊢SE phi.
+    Proof.
+      intros Hsat H.
+      assert (HA : ~ ~ (A ⊢SE ⊥ \/ ~ A ⊢SE ⊥)) by tauto.
+      apply HA. clear HA. intros [HA|HA].
+      - apply H. apply Absurd. assumption.
+      - specialize (Hsat _ K_std K_std_standard (exist cons A HA) ids).
+        apply K_std_sprv in Hsat.
+        + apply Hsat. intros Hsat'. apply H.
+          rewrite <- idSubst_form with ids phi; trivial.
+        + intros psi Hpsi. apply K_std_ksat.
+          intros B xi HB Hxi. asimpl in Hxi. eauto.
+    Qed.
+
+    Lemma K_std_seq_ksoundness A phi :
+      A ⊢SE phi -> A ⊫KS phi.
+    Proof.
+      intros H % seq_ND. apply @ksoundness with (b := expl). 2: apply H. firstorder.
+    Qed.
+  End StandardCompleteness.
+
+  (* *** MP is required *)
+
+  Section MPRequired.
+    Variable C : stab_class.
+    Hypothesis HC : map_closed C dnt.
+    Variable K_completeness : forall T phi, C T -> closed_T T -> closed phi -> kvalid_T kstandard T phi -> T ⊩SE phi.
+
+    Lemma cend_dn T phi :
+      closed_T T -> closed phi ->
+      C T -> ~ ~ T ⊩CE phi -> T ⊩CE phi.
+    Proof.
+      intros clT clphi HT Hdn. apply DN_T, dnt_to_TCE. cbn. apply (@seq_ND_T _ _ (tmap dnt T) (¬ (¬ dnt phi))). 
+      apply K_completeness. 1: apply HC, HT.
+      - intros ? ? (? & ? & <-). eapply dnt_unused. now eapply clT.
+      - intros n. repeat econstructor. eapply dnt_unused; eauto. 
+      - intros D M St u rho HT' v Hv Hn. contradict Hdn. intros Hphi % dnt_to_TIE.
+        apply strong_ksoundness with (C0 := kstandard) in Hphi. apply (St v), Hn. 1: reflexivity.
+        2: intros; apply kstandard_explodes. 1: apply (Hphi D M St v rho).
+        intros psi Hpsi % HT'. apply (ksat_mon Hv Hpsi).
+    Qed.
+  End MPRequired.
+  
+End KripkeCompleteness.
