theories/FOL/Deduction/FragmentSequent.v
@@ -1,0 +1,44 @@
+(** ** Normal Sequent Calculus **)
+
+From Undecidability Require Import Shared.ListAutomation.
+From Undecidability.Synthetic Require Import Definitions DecidabilityFacts EnumerabilityFacts ListEnumerabilityFacts ReducibilityFacts.
+Import ListAutomationNotations.
+From Undecidability Require Import FOL.Syntax.Facts.
+From Undecidability Require Import FOL.Syntax.Theories.
+Import FragmentSyntax.
+Export FragmentSyntax.
+
+Local Unset Implicit Arguments.
+Section Gentzen.
+
+  Context {Σ_funcs : funcs_signature}.
+  Context {Σ_preds : preds_signature}.
+
+  Inductive sprv : forall (b : falsity_flag), list form -> option form -> form -> Prop :=
+  | Contr {b} A phi psi : sprv b A (Some phi) psi -> phi el A -> sprv b A None psi
+  | IR {b} A phi psi : sprv b (phi :: A) None psi -> sprv b A None (phi → psi)
+  | AllR {b} A phi : sprv b (map (subst_form ↑) A) None phi -> sprv b A None (∀ phi)
+  | Absurd A phi : sprv falsity_on A None ⊥ -> sprv falsity_on A None phi
+  | Ax {b} A phi : sprv b A (Some phi) phi
+  | IL {b} A phi psi xi : sprv b A None phi -> sprv b A (Some psi) xi -> sprv b A (Some (phi → psi)) xi
+  | AllL {b} A phi t psi : sprv b A (Some (phi[t..])) psi -> sprv b A (Some (∀ phi)) psi.
+
+  Notation "A '⊢S' phi" := (sprv _ A None phi) (at level 30).
+  Notation "A ';;' phi '⊢s' psi" := (sprv _ A (Some phi) psi) (at level 70).
+  Arguments sprv {_} _ _ _.
+
+  Definition stprv {b : falsity_flag} (T : theory) (phi : form) : Prop :=
+    exists A, A ⊏ T /\ sprv A None phi.
+End Gentzen.
+
+#[global]
+Hint Constructors sprv : core.
+
+Notation "A '⊢S' phi" := (sprv _ A None phi) (at level 30).
+Notation "A ';;' phi '⊢s' psi" := (sprv _ A (Some phi) psi) (at level 70).
+Notation "A '⊢SE' phi" := (sprv falsity_on A None phi) (at level 30).
+Notation "A ';;' phi '⊢sE' psi" := (sprv falsity_on A (Some phi) psi) (at level 70). (*
+Notation "A '⊢SL' phi" := (sprv lconst A None phi) (at level 30).
+Notation "A ';;' phi '⊢sL' psi" := (sprv lconst A (Some phi) psi) (at level 70). *)
+Arguments sprv {_} {_} {_} _ _ _.
+Notation "T '⊩SE' phi" := (@stprv _ falsity_on T phi) (at level 30).
