theories/FOL/Deduction/FragmentSequentFacts.v
@@ -1,0 +1,287 @@
+(** ** Normal Sequent Calculus **)
+
+From Undecidability Require Import Shared.ListAutomation.
+From Undecidability.Synthetic Require Import Definitions DecidabilityFacts EnumerabilityFacts ListEnumerabilityFacts ReducibilityFacts.
+Import ListAutomationNotations.
+From Undecidability Require Import FOL.Syntax.Facts.
+From Undecidability Require Import FOL.Syntax.Theories.
+From Undecidability.FOL.Deduction Require Export FragmentSequent FragmentNDFacts.
+From Undecidability.FOL.Semantics.Kripke Require Import FragmentCore FragmentSoundness.
+Import FragmentSyntax.
+Export FragmentSyntax.
+
+Section Gentzen.
+
+  Context {Σ_funcs : funcs_signature}.
+  Context {Σ_preds : preds_signature}.
+
+  Lemma seq_consistent :
+    ~ [] ⊢S ⊥.
+  Proof.
+    enough (forall ff (H : falsity_on = ff), ~ [] ⊢S (match H in _ = f return @form _ _ _ f with eq_refl _ => ⊥ end)) as H.
+    - apply (H falsity_on eq_refl).
+    - intros ff Heq. remember nil. remember None.
+      remember (match _ with eq_refl _ => _ end).
+      intros H. induction H; subst; try intuition congruence.
+      now eapply IHsprv with eq_refl.
+  Qed.
+
+  Section Weakening.
+    Context {b : falsity_flag}.
+
+    Lemma seq_Weak A B phi psi :
+      sprv A phi psi -> A <<= B -> sprv B phi psi.
+    Proof.
+      intros H; induction H in B |-*; intuition; eauto using incl_map. 
+    Qed.
+
+    Theorem seq_subst_Weak A phi psi sigma :
+      sprv A phi psi -> sprv ([phi[sigma] | phi ∈ A]) (option_map (subst_form sigma) phi) psi[sigma].
+    Proof.
+      induction 1 in sigma |-*; cbn; eauto using in_map.
+      - apply AllR. setoid_rewrite map_map in IHsprv. erewrite map_map, map_ext.
+        apply IHsprv. intros ?. cbn. now rewrite up_form.
+      - specialize (IHsprv sigma). apply AllL with (t := t`[sigma]). cbn in IHsprv.
+        rewrite subst_comp in *. unfold scons, funcomp in *. erewrite subst_ext. apply IHsprv.
+        intros [|n]. 1: easy. cbn. unfold funcomp. rewrite subst_term_comp. apply subst_term_id.
+        easy.
+    Qed.
+
+    Context {HdF : eq_dec Σ_funcs} {HdP : eq_dec Σ_preds}.
+
+    Lemma seq_nameless_equiv_all' A phi n :
+      bounded_L n A -> bounded (S n) phi -> [f[↑] | f ∈ A] ⊢S phi <-> A ⊢S phi[$n..].
+    Proof.
+      intros HL Hphi. split.
+      - intros H. apply (seq_subst_Weak ($n..)) in H. rewrite map_map in *.
+        erewrite map_ext, map_id in H; try apply H. intros. apply subst_shift.
+      - intros H. apply (seq_subst_Weak (cycle_shift n)) in H.
+        rewrite (map_ext_in _ (subst_form ↑)) in H.
+        + now rewrite cycle_shift_subject in H.
+        + intros psi HP. now apply cycle_shift_shift, HL.
+    Qed.
+  End Weakening.
+
+  (* **** Normalization *)
+  Local Unset Implicit Arguments.
+  (* We redefine sprv and prv in Type so we define predicates on them. *)
+  Inductive tsprv : forall (b : falsity_flag), list form -> option form -> form -> Type :=
+  | TContr {b} A phi psi : tsprv b A (Some phi) psi -> phi el A -> tsprv b A None psi
+  | TIR {b} A phi psi : tsprv b (phi :: A) None psi -> tsprv b A None (phi → psi)
+  | TAllR {b} A phi : tsprv b (map (subst_form ↑) A) None phi -> tsprv b A None (∀ phi)
+  | TAbsurd A phi : tsprv falsity_on A None ⊥ -> tsprv falsity_on A None phi
+  | TAx {b} A phi : tsprv b A (Some phi) phi
+  | TIL {b} A phi psi xi : tsprv b A None phi -> tsprv b A (Some psi) xi -> tsprv b A (Some (phi → psi)) xi
+  | TAllL {b} A phi t psi : tsprv b A (Some (phi[t..])) psi -> tsprv b A (Some (∀ phi)) psi.
+  Arguments tsprv {_} _ _ _.
+
+  Inductive tprv : forall (b : falsity_flag), list (form) -> form -> Type :=
+  | TII {b} A phi psi : tprv b (phi::A) psi -> tprv b A (phi → psi)
+  | TIE {b} A phi psi : tprv b A (phi → psi) -> tprv b A phi -> tprv b A psi
+  | TAllI {b} A phi : tprv b (map (subst_form ↑) A) phi -> tprv b A (∀ phi)
+  | TAllE {b} A t phi : tprv b A (∀ phi) -> tprv b A (phi [t..])
+  | TExp A phi : tprv falsity_on A ⊥ -> tprv falsity_on A phi
+  | TCtx {b} A phi : phi el A -> tprv b A phi.
+  Arguments tprv {_} _ _.
+
+  Definition not_II {b : falsity_flag} {A} {phi} (p : tprv A phi) : Prop :=
+    match p with
+    | (TII _ _ _ p') => False
+    | (TAllI _ _ p') => True
+    | (TAllE _ _ _ p') => True
+    | (TExp _ _ p') => True
+    | (TIE _ _ _ p' p'') => True
+    | (TCtx _ _ _) => True
+    end.
+
+  Definition not_AllI {b : falsity_flag} {A} {phi} (p : tprv A phi) : Prop :=
+    match p with
+    | (TII _ _ _ p') => True
+    | (TAllI _ _ p') => False
+    | (TAllE _ _ _ p') => True
+    | (TExp _ _ p') => True
+    | (TIE _ _ _ p' p'') => True
+    | (TCtx _ _ _) => True
+    end.
+
+  Fixpoint normal {b : falsity_flag} {A} {phi} (p : tprv A phi) : Prop :=
+    match p with
+    | (TII _ _ _ p') => normal p'
+    | (TIE _ _ _ p' p'') => normal p' /\ normal p'' /\ not_II p'
+    | (TAllI _ _ p') => normal p'
+    | (TAllE _ _ _ p') => normal p' /\ not_AllI p'
+    | (TExp _ _ p') => normal p'
+    | (TCtx _ _ _) => True
+    end.
+
+  Section CutElimination.
+    Context {b : falsity_flag}.
+
+    Definition embed A phi psi :=
+      match phi with
+      | Some phi' => @prv _ _ _ intu A phi' -> @prv _ _ _ intu A psi
+      | None => @prv _ _ _ intu A psi
+      end.
+
+    Lemma seq_ND A phi psi :
+      sprv A phi psi -> embed A phi psi.
+    Proof.
+      unfold embed; induction 1; cbn in *.
+      - refine (IHsprv (Ctx H0)).
+      - refine (II IHsprv).
+      - refine (AllI IHsprv).
+      - refine (Exp phi IHsprv).
+      - tauto.
+      - intros. refine (IHsprv2 (IE H1 IHsprv1)).
+      - intros. refine (IHsprv (AllE t H0)).
+    Qed.
+
+    Lemma seq_ND_T T phi :
+      stprv T phi -> @FragmentND.tprv _ _ b intu T phi.
+    Proof.
+      intros (A & HA1 & HA2). apply seq_ND in HA2. now use_theory A.
+    Qed.
+
+    Definition tembed A phi psi :=
+      match phi with
+      | Some phi' => forall (p : tprv A phi'), not_AllI p /\ not_II p /\ normal p -> exists (p' : tprv A psi), normal p'
+      | None => exists (p : tprv A psi), normal p
+      end.
+
+    Lemma cutfree_seq_ND A phi psi :
+      tsprv A phi psi -> tembed A phi psi.
+    Proof with try split; cbn in *; unfold not_II, not_AllI in *; try tauto.
+      unfold tembed; induction 1; cbn in *.
+      - apply (IHX (TCtx _ _ i))...
+      - destruct IHX. exists (TII _ _ _ x)...
+      - destruct IHX. exists (TAllI _ _ x)...
+      - destruct IHX. exists (TExp _ phi x)...
+      - firstorder.
+      - intros. destruct IHX1. eapply (IHX2 (TIE _ _ _ p x))...
+      - intros. apply (IHX (TAllE _ t _ p))...
+    Qed.
+  End CutElimination.
+
+  Section Soundness.
+    Context {b : falsity_flag}.
+
+    Lemma ksoundness_seq A (phi : form) :
+      @sprv _ _ _ A None phi  -> kvalid_ctx A phi.
+    Proof.
+      intros Hprv % seq_ND. now apply ksoundness.
+    Qed.
+  End Soundness.
+
+  (* **** Enumerability of Sequents *)
+  Section Enumerability.
+  Variable list_Funcs : nat -> list syms.
+  Hypothesis enum_Funcs' : list_enumerator__T list_Funcs syms.
+
+  Variable list_Preds : nat -> list preds.
+  Hypothesis enum_Preds' : list_enumerator__T list_Preds preds.
+
+  Hypothesis eq_dec_Funcs : eq_dec syms.
+  Hypothesis eq_dec_Preds : eq_dec preds.
+
+  Instance eqdec_binop : eq_dec binop.
+  Proof.
+    intros x y. unfold dec. decide equality.
+  Qed.
+
+  Instance eqdec_quantop : eq_dec quantop.
+  Proof.
+    intros x y. unfold dec. decide equality.
+  Qed.
+
+  Definition list_binop (n : nat) := [Impl].
+
+  Instance enum_binop :
+    list_enumerator__T list_binop binop.
+  Proof.
+    intros []; exists 0; cbn; tauto.
+  Qed.
+
+  Definition list_quantop (n : nat) := [All].
+
+  Instance enum_quantop :
+    list_enumerator__T list_quantop quantop.
+  Proof.
+    intros []; exists 0; cbn; tauto.
+  Qed.
+
+  Lemma enumT_binop :
+    enumerable__T binop.
+  Proof.
+    apply enum_enumT. exists list_binop. apply enum_binop.
+  Qed.
+
+  Lemma enumT_quantop :
+    enumerable__T quantop.
+  Proof.
+    apply enum_enumT. exists list_quantop. apply enum_quantop.
+  Qed.
+
+  Instance enum_term' :
+    list_enumerator__T (L_term _) term :=
+    enum_term _.
+
+  Instance enum_form' {ff : falsity_flag} :
+    list_enumerator__T (L_form _ _ _ _) form :=
+    enum_form _ _ _ _.
+  Fixpoint L_seq {b : falsity_flag} (A : list form) (psi : option form) (n : nat) : list form :=
+    match n with
+    | 0 => match psi with Some psi => [psi] | None => A end
+    | S n => L_seq A psi n ++
+                  match psi with
+     (* Contr *)  | None => concat ([ L_seq A (Some psi) n | psi ∈ A]) ++
+     (* IR *)               concat ([ [ phi → psi | psi ∈ L_seq (phi :: A) None n ] | phi ∈ L_T form n]) ++
+     (* AllR *)             [ ∀ phi | phi ∈ L_seq ([ psi[↑] | psi ∈ A]) None n ] ++
+     (* Absurd *)           ((if b as ff return list (@form _ _ _ ff) -> list (@form _ _ _ ff)
+                              then fun _ => [] else fun A => [ phi | phi ∈ L_T form n, ⊥ el L_seq A None n ]) A)
+                  | Some psi' => match psi' in @form _ _ _ ff return list (@form _ _ _ ff) -> list (@form _ _ _ ff) with
+     (* IL *)         | @bin _ _ _ ff Impl phi psi => fun A => [ xi | xi ∈ L_seq A (Some psi) n, phi el @L_seq ff A None n ]
+     (* AllL *)       | quant All psi => fun A => concat ([ [phi | phi ∈ L_seq A (Some psi[t..]) n ] | t ∈ L_T term n])
+                      | _ => fun _ => [] end A
+                  end
+    end.
+
+    Opaque in_dec.
+
+    Lemma enum_sprv {b : falsity_flag} A psi : list_enumerator (L_seq A psi) (sprv A psi).
+    Proof with try (eapply cum_ge'; eauto; lia).
+      repeat split.
+      - rename x into phi. induction 1; try congruence; subst.
+        + destruct IHsprv as [m]. exists (S m). cbn. in_app 2.
+          eapply in_concat_iff. eexists. split. 2: in_collect phi... all: eauto.
+        + destruct IHsprv as [m1], (el_T phi) as [m2]. exists (1 + m1 + m2). cbn. in_app 3.
+          eapply in_concat_iff. eexists. split. 2: in_collect phi... in_collect psi...
+        + destruct IHsprv as [m]. exists (S m). cbn. in_app 4. in_collect phi...
+        + destruct IHsprv as [m1], (el_T phi) as [m2]. exists (1 + m1 + m2). cbn. in_app 5. in_collect phi...
+        + exists 0. now left.
+        + destruct IHsprv1 as [m1], IHsprv2 as [m2]. exists (1 + m1 + m2). cbn. in_app 2. in_collect xi...
+        + destruct IHsprv as [m1], (el_T t) as [m2]. exists (1 + m1 + m2). cbn. in_app 2. eapply in_concat_iff.
+          eexists. split. 2: in_collect t... in_collect psi...
+      - intros [m]. induction m in A, psi, x, H |-*; destruct psi; cbn in *.
+        + destruct H as [-> | []]. apply Ax.
+        + eauto.
+        + destruct f as [|b P v|b [] phi psi|b [] phi]; inv_collect; eauto.
+        + destruct b; inv_collect; eauto.
+    Qed.
+
+    Fixpoint L_tseq {b : falsity_flag} (L : nat -> list form) (n : nat) : list form :=
+      match n with
+      | 0 => nil
+      | S n => L_tseq L n ++ concat ([ L_seq A None n | A ∈ L_con L n ])
+      end.
+
+    Lemma enum_stprv {b : falsity_flag} T L : list_enumerator L T -> cumulative L -> list_enumerator (L_tseq L) (stprv T).
+    Proof with try (eapply cum_ge'; eauto; lia).
+      intros He Hcml psi. repeat split.
+      - intros (A & [m1] % (enum_el (enum_containsL Hcml He)) & [m2] % (enum_el (enum_sprv A None))).
+        exists (1 + (m1 + m2)). cbn. in_app 2. eapply in_concat_iff. eexists. split. 2: in_collect A... idtac...
+      - intros [m]. induction m in psi, H |-*; cbn in *. 1: contradiction. inv_collect. exists x0. split.
+        + eapply (enum_p (enum_containsL Hcml He)); eassumption.
+        + eapply (enum_p (enum_sprv x0 None)); eassumption.
+    Qed.
+  End Enumerability.
+End Gentzen.
