theories/FOL/Semantics/Kripke/FragmentSoundness.v
@@ -41,10 +41,61 @@ Section KSoundness.
     - now apply IHHprv in HA.
   Qed.
 
+  Lemma ksoundness_bot {ff1 ff2 : falsity_flag} A  (psi : @form _ _ _ ff1) (phi : @form _ _ _ ff2) :
+    closed psi ->
+    (forall xi, kvalid (psi → xi)) ->
+    A ⊢I phi -> kvalid_ctx (map (fun x => x [psi/⊥]) A) (phi[psi/⊥]).
+  Proof.
+    intros Hclosed Hexpl Hprv D M. remember intu as s. revert psi Hexpl Hclosed. induction Hprv; intros newbot Hexp Hclosed; subst; cbn; intros u rho HA.
+    all: repeat (clean_ksoundness + discriminate). all: (eauto || comp; eauto).
+    - intros v Hr Hpi. eapply IHHprv. 1-2:easy. intros ? []; subst; eauto using ksat_mon.
+    - eapply IHHprv1. 1-2:easy. 3: eapply IHHprv2. all: eauto. apply M.
+    - intros d. apply IHHprv. 1-2: now rewrite subst_closed. intros xi [psi' [<- [psi'' [<- Hpsi'']]%in_map_iff]] % in_map_iff.
+      rewrite <- subst_falsity_comm. rewrite ksat_comp. apply HA, in_map, Hpsi''.
+    - erewrite <- (subst_closed _ Hclosed). rewrite <- subst_falsity_comm.
+      rewrite ksat_comp. eapply ksat_ext.
+      2: {specialize (IHHprv newbot Hexp Hclosed).
+          rewrite subst_closed in IHHprv. 2:easy.
+          now eapply (IHHprv u rho HA (eval rho t)). } 
+      unfold funcomp. now intros [].
+    - apply (Hexp (phi[newbot/⊥]) D M u rho). 1: apply M. apply IHHprv. 1-2:easy. apply HA.
+  Qed.
+
+  Lemma ksoundness_bot_model {ff1 ff2 : falsity_flag} A  (psi : @form _ _ _ ff1) (phi : @form _ _ _ ff2) D (M : kmodel D):
+    closed psi ->
+    (ff2 = falsity_on -> forall u rho xi, rho ⊩(u,M) (psi → xi)) ->
+    A ⊢I phi -> 
+    forall u rho, 
+    (forall psi', psi' el (map (fun x => x [psi/⊥]) A) -> rho ⊩(u,M) psi') -> 
+    rho ⊩(u,M) (phi[psi/⊥]).
+  Proof.
+    intros Hclosed Hexpl Hprv. remember intu as s. revert psi Hexpl Hclosed. induction Hprv; intros newbot Hexp Hclosed; subst; cbn; intros u rho HA.
+    all: repeat (clean_ksoundness + discriminate). all: (eauto || comp; eauto).
+    - intros v Hr Hpi. eapply IHHprv. 1-2:easy. intros ? []; subst; eauto using ksat_mon.
+    - eapply IHHprv1. 1-2:easy. 3: eapply IHHprv2. all: eauto. apply M.
+    - intros d. apply IHHprv. 1-2: now rewrite subst_closed. intros xi [psi' [<- [psi'' [<- Hpsi'']]%in_map_iff]] % in_map_iff.
+      rewrite <- subst_falsity_comm. rewrite ksat_comp. apply HA, in_map, Hpsi''.
+    - erewrite <- (subst_closed _ Hclosed). rewrite <- subst_falsity_comm.
+      rewrite ksat_comp. eapply ksat_ext.
+      2: {specialize (IHHprv newbot Hexp Hclosed).
+          rewrite subst_closed in IHHprv. 2:easy.
+          now eapply (IHHprv u rho HA (eval rho t)). } 
+      unfold funcomp. now intros [].
+    - apply (Hexp u rho). 1: apply M. apply IHHprv. 1-2:easy. apply HA.
+  Qed.
+
   Lemma ksoundness' (phi : form) :
     [] ⊢I phi -> kvalid phi.
   Proof.
     intros H % ksoundness. firstorder.
+  Qed.
+
+  Lemma ksoundness'_bot {ff1 ff2 : falsity_flag} (psi : @form _ _ _ ff1) (phi : @form _ _ _ ff2) :
+    closed psi ->
+    (forall xi, kvalid (psi → xi)) ->
+    [] ⊢I phi -> kvalid (phi[psi/⊥]).
+  Proof.
+    intros Hcl Hexp H % (ksoundness_bot Hcl Hexp). intros D M u rho. now apply (H D M u rho).
   Qed.
 
 End KSoundness.
